theories/Semantics/IMP/Axiomatic.v
@@ -1,0 +1,196 @@
+From stdpp Require Import prelude.
+From sets Require Import Functions Ensemble.
+
+From Semantics Require Import Syntax State Eval.
+
+Inductive EAExp : Type :=
+    | LVar : nat -> EAExp
+    | EAVal : Z -> EAExp
+    | EVar : nat -> EAExp
+    | EPlus : EAExp -> EAExp -> EAExp
+    | EMinus : EAExp -> EAExp -> EAExp
+    | EMul : EAExp -> EAExp -> EAExp.
+
+Fixpoint aexp_to_eaexp (a : AExp) : EAExp :=
+  match a with
+  | AVal z => EAVal z
+  | Var x => EVar x
+  | Plus a1 a2 => EPlus (aexp_to_eaexp a1)  (aexp_to_eaexp a2)
+  | Minus a1 a2 => EMinus (aexp_to_eaexp a1)  (aexp_to_eaexp a2)
+  | Mul a1 a2 => EMul (aexp_to_eaexp a1)  (aexp_to_eaexp a2)
+  end.
+
+Coercion aexp_to_eaexp : AExp >-> EAExp.
+
+Inductive EBExp : Type :=
+    | EBVal : bool -> EBExp
+    | EAEq : EAExp -> EAExp -> EBExp
+    | EALe : EAExp -> EAExp -> EBExp
+    | ENot : EBExp -> EBExp
+    | EAnd : EBExp -> EBExp -> EBExp
+    | EOr : EBExp -> EBExp -> EBExp
+    | Forall : nat -> EBExp -> EBExp
+    .
+
+Definition eimpl (b1 b2: EBExp) : EBExp :=
+  EOr (ENot b1) b2.
+
+Fixpoint bexp_to_ebexp (b : BExp) : EBExp :=
+  match b with
+  | BVal t => EBVal t
+  | AEq a1 a2 => EAEq  (aexp_to_eaexp a1)  (aexp_to_eaexp a2)
+  | ALe a1 a2 => EALe  (aexp_to_eaexp a1)  (aexp_to_eaexp a2)
+  | Not b => ENot (bexp_to_ebexp b)
+  | And b1 b2 => EAnd (bexp_to_ebexp b1) (bexp_to_ebexp b2)
+  | Or b1 b2 => EOr (bexp_to_ebexp b1) (bexp_to_ebexp b2)
+  end.
+
+Coercion bexp_to_ebexp : BExp >-> EBExp.
+
+Definition substitution : Type := nat -> option AExp.
+
+Definition asubst (a : EAExp) (logv : substitution) (locv : substitution) : EAExp :=
+  (fix go (a : EAExp) :EAExp :=
+  match a with
+  | LVar x => default (LVar x) (aexp_to_eaexp <$> logv x)
+  | EAVal z => EAVal z
+  | EVar x => default (EVar x) (aexp_to_eaexp <$> locv x)
+  | EPlus a1 a2 => EPlus (go a1)  (go a2)
+  | EMinus a1 a2 => EMinus (go a1) (go a2)
+  | EMul a1 a2 => EMul (go a1)  (go a2)
+  end) a.
+
+Fixpoint bsubst  (b : EBExp) (logv : substitution) (locv : substitution) : EBExp :=
+  match b with
+  | EBVal t => EBVal t
+  | EAEq a1 a2 => EAEq (asubst a1 logv locv) (asubst a2 logv locv)
+  | EALe a1 a2 => EALe (asubst a1 logv locv) (asubst a2 logv locv)
+  | ENot b => ENot (bsubst b logv locv)
+  | EAnd b1 b2 => EAnd (bsubst b1 logv locv) (bsubst b2 logv locv)
+  | EOr b1 b2 => EOr (bsubst b1 logv locv) (bsubst b2 logv locv)
+  | Forall x b => Forall x (bsubst b (fn_update logv x None) locv)
+  end.
+
+Definition subst0 : substitution := const None.
+
+Definition update (subst : substitution) (sub : list (nat * AExp)) : substitution :=
+  foldr (fun p s => fn_update s p.1 (Some p.2)) subst sub.
+
+Definition eaeval (sigma : State) (I : nat -> Z): EAExp -> Z :=
+    fix eval (a : EAExp) :=
+    match a with
+    | LVar x => I x
+    | EAVal n => n
+    | EVar x => sigma x
+    | EPlus a1 a2 => (eval a1 + eval a2)%Z
+    | EMinus a1 a2 => (eval a1 - eval a2)%Z
+    | EMul a1 a2 => (eval a1 * eval a2)%Z
+    end.
+
+Lemma eaeval_aexp: forall (a : AExp) (sigma : State) (I : nat -> Z),
+    eaeval sigma I a = aeval sigma a.
+Proof.
+    intros.
+    induction a.
+    - done.
+    - done.
+    - by cbn; rewrite IHa1, IHa2.
+    - by cbn; rewrite IHa1, IHa2.
+    - by cbn; rewrite IHa1, IHa2.
+Qed.
+
+Lemma top_char X : X ≡ top True <-> I ∈ X.
+Proof.
+    rewrite elem_of_equiv_top.
+    split; [done |].
+    by intros HI [].
+Qed.
+
+Lemma bot_char (X : Ensemble True) : X ≡ ∅ <-> I ∉ X.
+Proof.
+    split; [by set_solver |].
+    intros HI.
+    apply equiv_empty.
+    by intros [] Hx.
+Qed.
+
+Lemma top_not_bottom : top True ≢ ∅.
+Proof.
+    rewrite bot_char.
+    by intro contra; apply contra.
+Qed.
+
+Fixpoint satsi_set (sigma I : State) (b : EBExp) : Ensemble True :=
+match b with
+| EBVal true => top True
+| EBVal false => ∅
+| EAEq a1 a2 => if decide (eaeval sigma I a1 = eaeval sigma I a2) then top True else ∅
+| EALe a1 a2 => if decide (eaeval sigma I a1 <= eaeval sigma I a2)%Z then top True else ∅
+| ENot b => complement (satsi_set sigma I b)
+| EAnd b1 b2 => (satsi_set sigma I b1) ∩ (satsi_set sigma I b2)
+| EOr b1 b2 => (satsi_set sigma I b1) ∪ (satsi_set sigma I b2)
+| Forall x b => indexed_intersection (fun z : Z => satsi_set sigma (fn_update I x z) b)
+end.
+
+Definition satsi (sigma I : State) (b : EBExp) : Prop :=
+    satsi_set sigma I b ≡ top True.
+
+Lemma satsi_true : forall (sigma I : State), satsi sigma I (BVal true).
+Proof. done. Qed.
+
+Lemma satsi_false : forall (sigma I : State), ~ satsi sigma I (BVal false).
+Proof.
+    intros sigma Interp; unfold satsi; cbn.
+    by intro contra; apply top_not_bottom.
+Qed.
+
+Lemma satsi_eq : forall (sigma I : State) (a1 a2 : EAExp),
+    satsi sigma I (EAEq a1 a2) <-> eaeval sigma I a1 = eaeval sigma I a2.
+Proof.
+    unfold satsi; cbn; split; intros; case_decide.
+    - done.
+    - by exfalso; apply top_not_bottom.
+    - done.
+    - done.
+Qed.
+
+Lemma satsi_le : forall (sigma I : State) (a1 a2 : EAExp),
+    satsi sigma I (EALe a1 a2) <-> (eaeval sigma I a1 <= eaeval sigma I a2)%Z.
+Proof.
+    unfold satsi; cbn; split; intros; case_decide.
+    - done.
+    - by exfalso; apply top_not_bottom.
+    - done.
+    - done.
+Qed.
+
+Lemma satsi_not : forall (sigma I : State) (b : EBExp),
+    satsi sigma I (ENot b) <-> ~ satsi sigma I b.
+Proof.
+    intros; unfold satsi; cbn.
+    by rewrite !top_char, elem_of_complement.
+Qed.
+
+Lemma satsi_and_intro : forall (sigma I : State) (b1 b2 : EBExp),
+     satsi sigma I b1 -> satsi sigma I b2 -> satsi sigma I (EAnd b1 b2).
+Proof. by set_solver. Qed.
+
+Lemma satsi_and_elim_l : forall (sigma I : State) (b1 b2 : EBExp),
+    satsi sigma I (EAnd b1 b2) -> satsi sigma I b1. 
+Proof. by set_solver. Qed.
+
+Lemma satsi_and_elim_r : forall (sigma I : State) (b1 b2 : EBExp),
+    satsi sigma I (EAnd b1 b2) -> satsi sigma I b2. 
+Proof. by set_solver. Qed.
+
+Lemma satsi_or : forall (sigma I : State) (b1 b2 : EBExp),
+    satsi sigma I (EOr b1 b2) <-> satsi sigma I b1 \/ satsi sigma I b2.
+Proof. by intros; unfold satsi; cbn; rewrite !top_char, elem_of_union. Qed.
+
+Lemma satsi_forall : forall (sigma I : State) (x : nat) (b : EBExp),
+    satsi sigma I (Forall x b) <-> forall (z : Z), satsi sigma (fn_update I x z) b.
+Proof.
+    intros; unfold satsi; cbn.
+    setoid_rewrite top_char.
+    by rewrite elem_of_indexed_intersection.
+Qed.
